.

src/program_proof/session/session_definitions.v
@@ -2,32 +2,70 @@ From Perennial.program_proof.session Require Export session_prelude.
 
 #[local] Tactic Notation "tac_val_t" :=
   let val := lazymatch goal with [ |- val_ty (?val _) _ ] => val end in
-  lazymatch goal with [ v : tuple_of ?tv |- _ ] =>
-    unfold tuple_of in v; unfold tv in v; simpl in v; unfold val; simpl SessionPrelude.value_of; repeat constructor; auto
-  end.
+  lazymatch goal with [ v : tuple_of ?tv |- _ ] => unfold tuple_of in v; unfold tv in v; simpl in v; unfold val; simpl SessionPrelude.value_of end;
+  repeat constructor; auto.
 
 #[local] Tactic Notation "tac_IntoVal" integer( n ) :=
   intros;
-  lazymatch goal with [ v : tuple_of ?tv |- _ ] =>
-    unfold tuple_of in v; unfold tv in v; simpl in v; simpl SessionPrelude.value_of;
-    do n destruct v as [v ?]; simpl
-  end;
+  lazymatch goal with [ v : tuple_of ?tv |- _ ] => unfold tuple_of in v; unfold tv in v; simpl in v; simpl SessionPrelude.value_of; do n destruct v as [v ?]; simpl end;
   repeat lazymatch goal with [ t : Slice.t |- _ ] => destruct t end; auto.
 
-Definition value_bound (a: Z) : u64 -> Prop :=
-  fun u: u64 => a >= 1 /\ uint.Z u ≤ 2 ^ 64 - a.
+#[universes(template)]
+Class has_value_boundary (t: Type) : Type :=
+  value_bound (a: Z) (object: t) : Prop.
+
+#[global] Hint Unfold value_bound : session_hints.
+
+#[global]
+Instance u64_has_value_boundary : has_value_boundary u64 :=
+  fun a: Z => fun u: u64 => a >= 1 /\ uint.Z u <= 2 ^ 64 - a.
+
+#[global]
+Instance nat_has_value_boundary : has_value_boundary nat :=
+  fun a: Z => fun n: nat => a >= 1 /\ Z.of_nat n <= 2 ^ 64 - a.
+  
+#[global]
+Instance list_has_value_boundary {t: Type} (t_has_value_boundary: has_value_boundary t) : has_value_boundary (list t) :=
+  fun a: Z => Forall ( @value_bound t t_has_value_boundary a).
+
+Module _Data.
+
+  Definition t : Type :=
+    u64.
+
+  #[global] Instance has_value_of_Data : SessionPrelude.has_value_of t :=
+    SessionPrelude.u64_has_value_of.
+
+  Definition ty : ty :=
+    uint64T.
+
+  Theorem val_ty v
+    : val_ty (SessionPrelude.u64_has_value_of v) _Data.ty.
+  Proof.
+    econstructor; auto.
+  Qed.
+
+  #[global] Hint Resolve _Data.val_ty : typeclasses_hints.
+
+  #[global]
+  Instance IntoVal : IntoVal _Data.t :=
+    u64_IntoVal.
+
+End _Data.
+
+#[local] Opaque _Data.t.
 
 Module Operation.
 
   Definition tv : TypeVector.t 2 :=
-    [Slice.t,u64].
+    [Slice.t,_Data.t].
 
   Definition from_val (v: val) : option (tuple_of tv) :=
     match v with
-    | (slice_v, (#(LitInt d), #()))%V =>
-      match slice_IntoVal.(from_val) slice_v with
-      | Some s => Some (s, d)
-      | None => None
+    | (VersionVector, (Data, #()))%V =>
+      match slice_IntoVal.(from_val) VersionVector, _Data.IntoVal.(from_val) Data with
+      | Some s1, Some d1 => Some (s1, d1)
+      | _, _ => None
       end
     | _ => None
     end.
@@ -35,31 +73,69 @@ Module Operation.
   Definition val (v: tuple_of tv) : val :=
     SessionPrelude.value_of v.
 
-  #[projections(primitive)]
-  Record t : Type := mk
+  #[projections(primitive), universes(template)]
+  Record t {u64: Type} : Type := mk
     { VersionVector: list u64
-    ; Data:          u64
+    ; Data:          _Data.t
     }.
 
-  Definition size_of (object: t) : nat :=
+  #[global] Arguments t : clear implicits. 
+
+  #[global]
+  Instance FMap
+    : FMap t.
+  Proof.
+    intros A B A_to_B F_A. econstructor.
+    - refine (fmap A_to_B _). refine (VersionVector _). exact F_A.
+    - refine (_). refine (Data _). exact F_A.
+  Defined.
+
+  Definition size_of {u64: Type} (object: t u64) : nat :=
     length object.(VersionVector).
 
-  Definition value_bound (a: Z) (object: t) : Prop :=
-    Forall (value_bound a) object.(VersionVector).
+  #[global]
+  Instance value_bound : has_value_boundary (t u64) :=
+    fun a: Z => fun object: t u64 => value_bound a object.(VersionVector).
+
+  Section ADD_ON.
+
+    Context {u64: Type}.
+
+    Definition getVersionVector (op: Operation.t u64) : list u64 :=
+      op.(VersionVector).
+
+    Context {u64_well_formed: u64 -> Prop}.
+
+    Definition well_formed (n: nat) (op: Operation.t u64) : Prop :=
+      Forall u64_well_formed op.(VersionVector) /\ length op.(VersionVector) = n.
+
+    Context {u64_hsEq: SessionPrelude.hsEq u64 (well_formed := u64_well_formed)}.
+
+    #[global]
+    Instance hsEq_Operation (n: nat) : SessionPrelude.hsEq (Operation.t u64) (well_formed := well_formed n) :=
+      SessionPrelude.hsEq_preimage getVersionVector.
+
+    Context {u64_hsOrd: SessionPrelude.hsOrd u64 (well_formed := u64_well_formed)}.
+
+    #[global]
+    Instance hsOrd_Operation (n: nat) : SessionPrelude.hsOrd (Operation.t u64) (well_formed := well_formed n) :=
+      SessionPrelude.hsOrd_preimage getVersionVector.
+
+  End ADD_ON.
 
 End Operation.
 
 Module Message.
 
   Definition tv : TypeVector.t 18 :=
-    [u64,u64,u64,u64,u64,Slice.t,u64,u64,Slice.t,u64,u64,u64,u64,u64,u64,Slice.t,u64,u64].
+    [u64,u64,u64,u64,_Data.t,Slice.t,u64,u64,Slice.t,u64,u64,u64,u64,u64,_Data.t,Slice.t,u64,u64].
 
   Definition from_val (v: val) : option (tuple_of tv) :=
     match v with
-    | (#(LitInt MessageType), (#(LitInt C2S_Client_Id), (#(LitInt C2S_Server_Id), (#(LitInt C2S_Client_OperationType), (#(LitInt C2S_Client_Data), (C2S_Client_VersionVector, (#(LitInt S2S_Gossip_Sending_ServerId), (#(LitInt S2S_Gossip_Receiving_ServerId), (S2S_Gossip_Operations, (#(LitInt S2S_Gossip_Index), (#(LitInt S2S_Acknowledge_Gossip_Sending_ServerId), (#(LitInt S2S_Acknowledge_Gossip_Receiving_ServerId), (#(LitInt S2S_Acknowledge_Gossip_Index), (#(LitInt S2C_Client_OperationType), (#(LitInt S2C_Client_Data), (S2C_Client_VersionVector, (#(LitInt S2C_Server_Id), (#(LitInt S2C_Client_Number), #()))))))))))))))))))%V =>
-      match slice_IntoVal.(from_val) C2S_Client_VersionVector, slice_IntoVal.(from_val) S2S_Gossip_Operations, slice_IntoVal.(from_val) S2C_Client_VersionVector with
-      | Some s1, Some s2, Some s3 => Some (MessageType, C2S_Client_Id, C2S_Server_Id, C2S_Client_OperationType, C2S_Client_Data, s1, S2S_Gossip_Sending_ServerId, S2S_Gossip_Receiving_ServerId, s2, S2S_Gossip_Index, S2S_Acknowledge_Gossip_Sending_ServerId, S2S_Acknowledge_Gossip_Receiving_ServerId, S2S_Acknowledge_Gossip_Index, S2C_Client_OperationType, S2C_Client_Data, s3, S2C_Server_Id, S2C_Client_Number)
-      | _, _, _ => None
+    | (#(LitInt MessageType), (#(LitInt C2S_Client_Id), (#(LitInt C2S_Server_Id), (#(LitInt C2S_Client_OperationType), (C2S_Client_Data, (C2S_Client_VersionVector, (#(LitInt S2S_Gossip_Sending_ServerId), (#(LitInt S2S_Gossip_Receiving_ServerId), (S2S_Gossip_Operations, (#(LitInt S2S_Gossip_Index), (#(LitInt S2S_Acknowledge_Gossip_Sending_ServerId), (#(LitInt S2S_Acknowledge_Gossip_Receiving_ServerId), (#(LitInt S2S_Acknowledge_Gossip_Index), (#(LitInt S2C_Client_OperationType), (S2C_Client_Data, (S2C_Client_VersionVector, (#(LitInt S2C_Server_Id), (#(LitInt S2C_Client_Number), #()))))))))))))))))))%V =>
+      match slice_IntoVal.(from_val) C2S_Client_VersionVector, slice_IntoVal.(from_val) S2S_Gossip_Operations, slice_IntoVal.(from_val) S2C_Client_VersionVector, _Data.IntoVal.(from_val) C2S_Client_Data, _Data.IntoVal.(from_val) S2C_Client_Data with
+      | Some s1, Some s2, Some s3, Some d1, Some d2 => Some (MessageType, C2S_Client_Id, C2S_Server_Id, C2S_Client_OperationType, d1, s1, S2S_Gossip_Sending_ServerId, S2S_Gossip_Receiving_ServerId, s2, S2S_Gossip_Index, S2S_Acknowledge_Gossip_Sending_ServerId, S2S_Acknowledge_Gossip_Receiving_ServerId, S2S_Acknowledge_Gossip_Index, S2C_Client_OperationType, d2, s3, S2C_Server_Id, S2C_Client_Number)
+      | _, _, _, _, _ => None
       end
     | _ => None
     end.
@@ -67,19 +143,19 @@ Module Message.
   Definition val (v: tuple_of tv) : val :=
     SessionPrelude.value_of v.
 
-  #[projections(primitive)]
-  Record t : Type := mk
+  #[projections(primitive), universes(template)]
+  Record t {u64: Type} : Type := mk
     { MessageType:  u64
 
     ; C2S_Client_Id:            u64
     ; C2S_Server_Id:            u64
     ; C2S_Client_OperationType: u64
-    ; C2S_Client_Data:          u64
+    ; C2S_Client_Data:          _Data.t
     ; C2S_Client_VersionVector: list u64
 
     ; S2S_Gossip_Sending_ServerId:   u64
     ; S2S_Gossip_Receiving_ServerId: u64
-    ; S2S_Gossip_Operations:         list Operation.t
+    ; S2S_Gossip_Operations:         list (Operation.t u64)
     ; S2S_Gossip_Index:              u64
 
     ; S2S_Acknowledge_Gossip_Sending_ServerId:   u64
@@ -87,18 +163,62 @@ Module Message.
     ; S2S_Acknowledge_Gossip_Index:              u64
 
     ; S2C_Client_OperationType: u64
-    ; S2C_Client_Data:          u64
+    ; S2C_Client_Data:          _Data.t
     ; S2C_Client_VersionVector: list u64
     ; S2C_Server_Id:            u64
     ; S2C_Client_Number:        u64
     }.
 
-  Definition size_of (object: t) : nat * nat :=
+  #[global] Arguments t : clear implicits.
+
+  #[global]
+  Instance FMap
+    : FMap t.
+  Proof.
+    intros A B A_to_B F_A. econstructor.
+    - refine (A_to_B _). refine (MessageType _). exact F_A.
+    - refine (A_to_B _). refine (C2S_Client_Id _). exact F_A.
+    - refine (A_to_B _). refine (C2S_Server_Id _). exact F_A.
+    - refine (A_to_B _). refine (C2S_Client_OperationType _). exact F_A.
+    - refine (_). refine (C2S_Client_Data _). exact F_A.
+    - refine (fmap A_to_B _). refine (C2S_Client_VersionVector _). exact F_A.
+    - refine (A_to_B _). refine (S2S_Gossip_Sending_ServerId _). exact F_A.
+    - refine (A_to_B _). refine (S2S_Gossip_Receiving_ServerId _). exact F_A.
+    - refine (fmap (Operation.FMap A B A_to_B) _). refine (S2S_Gossip_Operations _). exact F_A.
+    - refine (A_to_B _). refine (S2S_Gossip_Index _). exact F_A.
+    - refine (A_to_B _). refine (S2S_Acknowledge_Gossip_Sending_ServerId _). exact F_A.
+    - refine (A_to_B _). refine (S2S_Acknowledge_Gossip_Receiving_ServerId _). exact F_A.
+    - refine (A_to_B _). refine (S2S_Acknowledge_Gossip_Index _). exact F_A.
+    - refine (A_to_B _). refine (S2C_Client_OperationType _). exact F_A.
+    - refine (_). refine (S2C_Client_Data _). exact F_A.
+    - refine (fmap A_to_B _). refine (S2C_Client_VersionVector _). exact F_A.
+    - refine (A_to_B _). refine (S2C_Server_Id _). exact F_A.
+    - refine (A_to_B _). refine (S2C_Client_Number _). exact F_A.
+  Defined.
+
+  Definition size_of (object: t u64) : nat * nat :=
     (length object.(C2S_Client_VersionVector), length object.(S2C_Client_VersionVector)).
 
-  Definition value_bound (a: Z) (object: t) : Prop.
-    (* TODO *)
-  Admitted.
+  Variant _value_bound {a: Z} (object: t u64) : Prop :=
+    | _value_bound_intro
+      (C2S_Client_Id_bound: value_bound a object.(C2S_Client_Id))
+      (C2S_Server_Id_bound: value_bound a object.(C2S_Server_Id))
+      (C2S_Client_VersionVector: value_bound a object.(C2S_Client_VersionVector))
+      (S2S_Gossip_Sending_ServerId_bound: value_bound a object.(S2S_Gossip_Sending_ServerId))
+      (S2S_Gossip_Receiving_ServerId_bound: value_bound a object.(S2S_Gossip_Receiving_ServerId))
+      (S2S_Gossip_Operations_bound: value_bound a object.(S2S_Gossip_Operations))
+      (S2S_Gossip_Index_bound: value_bound a object.(S2S_Gossip_Index))
+      (S2S_Acknowledge_Gossip_Sending_ServerId_bound: value_bound a object.(S2S_Acknowledge_Gossip_Sending_ServerId))
+      (S2S_Acknowledge_Gossip_Receiving_ServerId_bound: value_bound a object.(S2S_Acknowledge_Gossip_Receiving_ServerId))
+      (S2S_Acknowledge_Gossip_Index_bound: value_bound a object.(S2S_Acknowledge_Gossip_Index))
+      (S2C_Client_VersionVector_bound: value_bound a object.(S2C_Client_VersionVector))
+      (S2C_Server_Id_bound: value_bound a object.(S2C_Server_Id))
+      (S2C_Client_Number: value_bound a object.(S2C_Client_Number))
+      : _value_bound object.
+
+  #[global]
+  Instance has_value_boundary : has_value_boundary (t u64) :=
+    @_value_bound.
 
 End Message.
 
@@ -120,24 +240,53 @@ Module Server.
   Definition val (v: tuple_of tv) : val :=
     SessionPrelude.value_of v.
 
-  #[projections(primitive)]
-  Record t : Type := mk
+  #[projections(primitive), universes(template)]
+  Record t {u64: Type} : Type := mk
     { Id:                     u64
     ; NumberOfServers:        u64
-    ; UnsatisfiedRequests:    list Message.t
+    ; UnsatisfiedRequests:    list (Message.t u64)
     ; VectorClock:            list u64
-    ; OperationsPerformed:    list Operation.t
-    ; MyOperations:           list Operation.t
-    ; PendingOperations:      list Operation.t
+    ; OperationsPerformed:    list (Operation.t u64)
+    ; MyOperations:           list (Operation.t u64)
+    ; PendingOperations:      list (Operation.t u64)
     ; GossipAcknowledgements: list u64
     }.
 
-  Definition size_of (object: t) : nat * nat * nat * nat * nat :=
+  #[global] Arguments t : clear implicits.
+
+  #[global]
+  Instance FMap
+    : FMap Server.t.
+  Proof.
+    intros A B A_to_B F_A. econstructor.
+    - refine (A_to_B _). refine (Id _). exact F_A.
+    - refine (A_to_B _). refine (NumberOfServers _). exact F_A.
+    - refine (fmap (Message.FMap A B A_to_B) _). refine (UnsatisfiedRequests _). exact F_A.
+    - refine (fmap A_to_B _). refine (VectorClock _). exact F_A.
+    - refine (fmap (Operation.FMap A B A_to_B) _). refine (OperationsPerformed _). exact F_A.
+    - refine (fmap (Operation.FMap A B A_to_B) _). refine (MyOperations _). exact F_A.
+    - refine (fmap (Operation.FMap A B A_to_B) _). refine (PendingOperations _). exact F_A.
+    - refine (fmap A_to_B _). refine (GossipAcknowledgements _). exact F_A.
+  Qed.
+
+  Definition size_of (object: t u64) : nat * nat * nat * nat * nat :=
     (length object.(VectorClock), length object.(OperationsPerformed), length object.(MyOperations), length object.(PendingOperations), length object.(GossipAcknowledgements)).
 
-  Definition value_bound (a: Z) (object: t) : Prop.
-    (* TODO *)
-  Admitted.
+  Variant _value_bound {a: Z} (object: t u64) : Prop :=
+    | _value_bound_intro
+      (Id_bound: value_bound a object.(Id))
+      (NumberOfServers_bound: value_bound a object.(NumberOfServers))
+      (UnsatisfiedRequests_bound: value_bound a object.(UnsatisfiedRequests))
+      (VectorClock_bound: value_bound a object.(VectorClock))
+      (OperationsPerformed_bound: value_bound a object.(OperationsPerformed))
+      (MyOperations_bound: value_bound a object.(MyOperations))
+      (PendingOperations_bound: value_bound a object.(PendingOperations))
+      (GossipAcknowledgements_bound: value_bound a object.(GossipAcknowledgements))
+      : _value_bound object.
+
+  #[global]
+  Instance has_value_boundary : has_value_boundary (t u64) :=
+    @_value_bound.
 
 End Server.
 
@@ -159,8 +308,8 @@ Module Client.
   Definition val (v: tuple_of tv) : val :=
     SessionPrelude.value_of v.
 
-  #[projections(primitive)]
-  Record t : Type := mk
+  #[projections(primitive), universes(template)]
+  Record t {u64: Type} : Type := mk
     { Id:                 u64
     ; NumberOfServers:    u64
     ; WriteVersionVector: list u64
@@ -168,12 +317,34 @@ Module Client.
     ; SessionSemantic:    u64
     }.
 
-  Definition size_of (object: t) : nat * nat :=
+  #[global] Arguments t : clear implicits.
+
+  #[global]
+  Instance FMap
+    : FMap Client.t.
+  Proof.
+    intros A B A_to_B F_A. econstructor.
+    - refine (A_to_B _). refine (Id _). exact F_A.
+    - refine (A_to_B _). refine (NumberOfServers _). exact F_A.
+    - refine (fmap A_to_B _). refine (WriteVersionVector _). exact F_A.
+    - refine (fmap A_to_B _). refine (ReadVersionVector _). exact F_A.
+    - refine (A_to_B _). refine (SessionSemantic _). exact F_A.
+  Defined.
+
+  Definition size_of (object: t u64) : nat * nat :=
     (length object.(WriteVersionVector), length object.(ReadVersionVector)).
 
-  Definition value_bound (a: Z) (object: t) : Prop.
-    (* TODO *)
-  Admitted.
+  Variant _value_bound {a: Z} (object: t u64) : Prop :=
+    | _value_bound_intro
+      (Id_bound: value_bound a object.(Id))
+      (NumberOfServers_bound: value_bound a object.(NumberOfServers))
+      (WriteVersionVector_bound: value_bound a object.(WriteVersionVector))
+      (ReadVersionVector_bound: value_bound a object.(ReadVersionVector))
+      : _value_bound object.
+
+  #[global]
+  Instance has_value_boundary : has_value_boundary (t u64) :=
+    @_value_bound.
 
 End Client.
 
@@ -182,7 +353,7 @@ Module ServerSide.
   Include SessionServer.
 
   Theorem Operation_val_t v
-    : val_ty (Operation.val v) (struct.t Operation).
+    : val_ty (Operation.val v) (struct.t SessionServer.Operation).
   Proof.
     tac_val_t.
   Qed.
@@ -197,14 +368,14 @@ Module ServerSide.
       {|
         to_val := Operation.val;
         from_val := Operation.from_val;
-        IntoVal_def := (IntoVal_def Slice.t, W64 0);
+        IntoVal_def := (IntoVal_def Slice.t, IntoVal_def _Data.t);
       |}
     ).
     tac_IntoVal 1.
   Defined.
 
   Theorem Message_val_t v
-    : val_ty (Message.val v) (struct.t Message).
+    : val_ty (Message.val v) (struct.t SessionServer.Message).
   Proof.
     tac_val_t.
   Qed.
@@ -219,14 +390,14 @@ Module ServerSide.
       {|
         to_val := Message.val;
         from_val := Message.from_val;
-        IntoVal_def := (W64 0, W64 0, W64 0, W64 0, W64 0, IntoVal_def Slice.t, W64 0, W64 0, IntoVal_def Slice.t, W64 0, W64 0, W64 0, W64 0, W64 0, W64 0, IntoVal_def Slice.t, W64 0, W64 0);
+        IntoVal_def := (W64 0, W64 0, W64 0, W64 0, IntoVal_def _Data.t, IntoVal_def Slice.t, W64 0, W64 0, IntoVal_def Slice.t, W64 0, W64 0, W64 0, W64 0, W64 0, IntoVal_def _Data.t, IntoVal_def Slice.t, W64 0, W64 0);
       |}
     ).
     tac_IntoVal 17.
   Defined.
 
   Theorem Server_val_t v
-    : val_ty (Server.val v) (struct.t Server).
+    : val_ty (Server.val v) (struct.t SessionServer.Server).
   Proof.
     tac_val_t.
   Qed.
@@ -244,22 +415,22 @@ Module ServerSide.
         IntoVal_def := (W64 0, W64 0, IntoVal_def Slice.t, IntoVal_def Slice.t, IntoVal_def Slice.t, IntoVal_def Slice.t, IntoVal_def Slice.t, IntoVal_def Slice.t);
       |}
     ).
-    tac_IntoVal 8.
+    tac_IntoVal 7.
   Defined.
 
   Section heap.
 
     Context `{hG: !heapGS Σ}.
 
-    Definition is_good_operation (v: tuple_of Operation.tv) (object: Operation.t) (n: nat) : iProp Σ :=
+    Definition is_good_operation (v: tuple_of Operation.tv) (object: Operation.t u64) (n: nat) : iProp Σ :=
       own_slice_small v!(0) uint64T DfracDiscarded object.(Operation.VersionVector) ∗
       ⌜v!(1) = object.(Operation.Data)⌝ ∗
       ⌜Operation.size_of object = n⌝.
 
-    Definition is_good_slice_of_operations (s: Slice.t) (objects: list Operation.t) (n: nat) : iProp Σ :=
+    Definition is_good_slice_of_operations (s: Slice.t) (objects: list (Operation.t u64)) (n: nat) : iProp Σ :=
       ∃ vs, own_slice s (struct.t Operation) (DfracOwn 1) vs ∗ [∗ list] v;o ∈ vs;objects, is_good_operation v o n.
 
-    Definition is_good_message (v: tuple_of Message.tv) (object: Message.t) (n: nat) (len_c2s: nat) (len_s2c: nat) : iProp Σ :=
+    Definition is_good_message (v: tuple_of Message.tv) (object: Message.t u64) (n: nat) (len_c2s: nat) (len_s2c: nat) : iProp Σ :=
       ⌜v!(0) = object.(Message.MessageType)⌝ ∗
       ⌜v!(1) = object.(Message.C2S_Client_Id)⌝ ∗
       ⌜v!(2) = object.(Message.C2S_Server_Id)⌝ ∗
@@ -281,10 +452,10 @@ Module ServerSide.
       ⌜v!(17) = object.(Message.S2C_Client_Number)⌝ ∗
       ⌜Message.size_of object = (len_c2s, len_s2c)⌝.
 
-    Definition is_good_slice_of_messages (s: Slice.t) (objects: list Message.t) (n: nat) (len_c2s: nat) : iProp Σ :=
+    Definition is_good_slice_of_messages (s: Slice.t) (objects: list (Message.t u64)) (n: nat) (len_c2s: nat) : iProp Σ :=
       ∃ vs, own_slice s (struct.t Message) (DfracOwn 1) vs ∗ [∗ list] v;o ∈ vs;objects, ∃ len_s2c : nat, is_good_message v o n len_c2s len_s2c.
 
-    Definition is_good_server' {OWN_UnsatisfiedRequests: bool} (v: tuple_of Server.tv) (object: Server.t) (n: nat) (len_vc: nat) (len_op: nat) (len_mo: nat) (len_po: nat) (len_ga: nat) : iProp Σ :=
+    Definition is_good_server' {OWN_UnsatisfiedRequests: bool} (v: tuple_of Server.tv) (object: Server.t u64) (n: nat) (len_vc: nat) (len_op: nat) (len_mo: nat) (len_po: nat) (len_ga: nat) : iProp Σ :=
       ⌜v!(0) = object.(Server.Id)⌝ ∗
       ⌜v!(1) = object.(Server.NumberOfServers)⌝ ∗
       (if OWN_UnsatisfiedRequests then is_good_slice_of_messages v!(2) object.(Server.UnsatisfiedRequests) n len_vc else emp)%I ∗
@@ -295,10 +466,9 @@ Module ServerSide.
       own_slice_small v!(7) uint64T (DfracOwn 1) object.(Server.GossipAcknowledgements) ∗
       ⌜Server.size_of object = (len_vc, len_op, len_mo, len_po, len_ga)⌝.
 
-    Definition is_good_server :=
-      is_good_server' (OWN_UnsatisfiedRequests := true).
-
   End heap.
+
+  Notation is_good_server := (is_good_server' (OWN_UnsatisfiedRequests := true)).
 
   Section Coq_nat.
 
@@ -313,7 +483,7 @@ Module ClientSide.
   Include SessionClient.
 
   Theorem Operation_val_t v
-    : val_ty (Operation.val v) (struct.t Operation).
+    : val_ty (Operation.val v) (struct.t SessionClient.Operation).
   Proof.
     exact (ServerSide.Operation_val_t v).
   Defined.
@@ -328,7 +498,7 @@ Module ClientSide.
   Defined.
 
   Theorem Message_val_t v
-    : val_ty (Message.val v) (struct.t Message).
+    : val_ty (Message.val v) (struct.t SessionClient.Message).
   Proof.
     exact (ServerSide.Message_val_t v).
   Defined.
@@ -343,7 +513,7 @@ Module ClientSide.
   Defined.
 
   Theorem Client_val_t v
-    : val_ty (Client.val v) (struct.t Client).
+    : val_ty (Client.val v) (struct.t SessionClient.Client).
   Proof.
     tac_val_t.
   Defined.
@@ -364,23 +534,19 @@ Module ClientSide.
     tac_IntoVal 4.
   Defined.
 
+  Notation is_good_operation := ServerSide.is_good_operation.
+
+  Notation is_good_slice_of_operations := ServerSide.is_good_slice_of_operations.
+
+  Notation is_good_message := ServerSide.is_good_message.
+
+  Notation is_good_slice_of_messages := ServerSide.is_good_slice_of_messages.
+
   Section heap.
 
     Context `{hG: !heapGS Σ}.
 
-    Definition is_good_operation :=
-      ServerSide.is_good_operation.
-
-    Definition is_good_slice_of_operations :=
-      ServerSide.is_good_slice_of_operations.
-
-    Definition is_good_message :=
-      ServerSide.is_good_message.
-
-    Definition is_good_slice_of_messages :=
-      ServerSide.is_good_slice_of_messages.
-
-    Definition is_good_client (v: tuple_of Client.tv) (object: Client.t) (n: nat) : iProp Σ :=
+    Definition is_good_client (v: tuple_of Client.tv) (object: Client.t u64) (n: nat) : iProp Σ :=
       ⌜v!(0) = object.(Client.Id)⌝ ∗
       ⌜v!(1) = object.(Client.NumberOfServers)⌝ ∗
       own_slice_small v!(2) uint64T (DfracOwn 1) object.(Client.WriteVersionVector) ∗
@@ -391,6 +557,8 @@ Module ClientSide.
   End heap.
 
   Section Coq_nat.
+
+    Import ServerSide.
 
     (* TODO *)
 
@@ -404,6 +572,25 @@ Section heap.
 
   Context `{hG: !heapGS Σ}.
 
-  (* TODO *)
+  Lemma Operation_well_formed (n: nat) v op
+    : (is_good_operation v op n)%I ⊢@{iProp Σ} (⌜Operation.well_formed (u64_well_formed := fun _ : u64 => True) n op⌝)%I.
+  Proof.
+    iIntros "H_hd". iDestruct "H_hd" as "(H3 & %H2 & %H1)"; iClear "H3".
+    iPureIntro; split; [eapply SessionPrelude.Forall_True | done].
+  Qed.
+
+  Lemma Forall_Operation_well_formed (n: nat) vs ops
+    : ([∗ list] v;op ∈ vs;ops, is_good_operation v op n)%I ⊢@{iProp Σ} (⌜Forall (Operation.well_formed (u64_well_formed := fun _ : u64 => True) n) ops⌝)%I.
+  Proof.
+    revert vs; induction ops as [ | hd tl IH]; intros vs.
+    - iIntros "H_big_sepL2"; iPureIntro; eauto.
+    - iIntros "H_big_sepL2".
+      iPoseProof (big_sepL2_cons_inv_r with "H_big_sepL2") as "(%hd' & %tl' & -> & H_hd & H_tl)".
+      iAssert (⌜Operation.well_formed n hd⌝)%I as "%YES1".
+      { iApply Operation_well_formed. iExact "H_hd". }
+      iAssert (⌜Forall (Operation.well_formed n) tl⌝)%I as "%YES2".
+      { iApply IH; iExact "H_tl". }
+      iPureIntro; econstructor; trivial.
+  Qed.
 
 End heap.
